feat: WSat (#303)
Co-authored-by: Markus de Medeiros <markusdemedeiros@outlook.com>

src/Iris/Std/PartialMap.lean
@@ -7,7 +7,7 @@ module
 
 import Batteries.Data.List.Perm
 import Iris.Std.FromMathlib
-
+public import Iris.Std.GenSets
 
 /-! ## Partial Maps
 
@@ -246,6 +246,9 @@ def mapFold {A : Type _} (f : K → V → A → A) (a : A) (m : M V) : A :=
 /-- Convert a list to a map with sequential natural number keys starting from `start`. -/
 def map_seq [FiniteMap M Nat] (start : Nat) (l : List V) : M V :=
   PartialMap.ofList (l.mapIdx (fun i v => (start + i, v)))
+
+def dom_set [LawfulSet S K] (m : M V) : S :=
+  LawfulSet.ofList (mapFold (fun k _ acc => k :: acc) [] m)
 
 end FiniteMap
 
@@ -1063,6 +1066,11 @@ theorem toList_zip {m₁ : M V} {m₂ : M V'} :
     obtain ⟨b, Hb₁, rfl, rfl⟩ := Ha₂
     refine ⟨a.2, toList_get.mp Ha₁, ?_⟩
     simp [Hb₁]
+
+theorem mem_dom_set [LawfulSet S K] {m : M V} : k ∈ (dom_set m : S) ↔ (get? m k).isSome := by
+  simp [dom_set, ←LawfulSet.mem_ofList, FiniteMap.mapFold, Option.isSome_iff_exists,
+    ←LawfulFiniteMap.toList_get]
+  rfl
 
 end LawfulFiniteMap
 
