src/Iris/Std/Positives.lean
@@ -98,6 +98,16 @@ def toNat : Pos → Nat
 
 instance : CoeOut Pos Nat where coe := Pos.toNat
 
+theorem Pos_toNat_pos (a : Pos) : 0 < a.toNat := by
+  induction a with
+  | xH => simp [Pos.toNat]
+  | xI a' ih => simp [Pos.toNat]
+  | xO a' ih => simp [Pos.toNat]; omega
+
+theorem Pos_toNat_inj {a b : Pos} (h : a.toNat = b.toNat) : a = b := by
+  induction a generalizing b <;> cases b
+  all_goals simp [Pos.toNat] at h; grind [Pos_toNat_pos]
+
 def compare (a b : Pos) : Ordering :=
   Ord.compare (a.toNat) (b.toNat)
 
@@ -356,5 +366,26 @@ instance : Countable Pos where
   encode := id
   decode := some
   decode_encode _ := rfl
+
+instance : Ord Pos where
+  compare x y := Pos.compare x y
+
+instance : Std.TransOrd Pos where
+  eq_swap {a b} := by
+    simp only [Ord.compare, Pos.compare]
+    rw [compareOfLessAndEq_eq_swap] <;> omega
+  isLE_trans {a b c} := by
+    have heq : ∀ {x y}, (compareOfLessAndEq x y).isLE = true ↔ x ≤ y :=
+      isLE_compareOfLessAndEq Nat.le_antisymm Nat.not_le Nat.le_total
+    simp only [Ord.compare, Pos.compare, heq]
+    grind
+
+instance : Std.LawfulEqOrd Pos where
+  eq_of_compare {a b} := by
+    simp only [Ord.compare, compare]
+    rw [compareOfLessAndEq_eq_eq Nat.le_refl (by grind)]
+    exact Pos_toNat_inj
+  compare_self {_} := by
+    simp [Ord.compare, Pos.compare, compareOfLessAndEq_eq_eq]
 
 end Pos
